coq/BitsToLists.v
@@ -1,0 +1,1256 @@
+Require Export Koika.Common Koika.Environments Koika.ULogs Koika.Syntax
+        Koika.Syntax.
+
+
+Ltac destr_in H :=
+  match type of H with
+  | context[match ?a with _ => _ end] => destruct a eqn:?
+  end.
+
+Ltac destr :=
+  match goal with
+    |- context[match ?a with _ => _ end] => destruct a eqn:?; try congruence
+  end.
+
+Ltac inv H :=
+  inversion H; try subst; clear H.
+
+Inductive val :=
+| Bits (sz:nat) (v: list bool)
+| Enum (sig: enum_sig) (v: list bool)
+| Struct (sig: struct_sig) (v: list val)
+| Array (sig: array_sig) (v: list val).
+
+
+    Fixpoint val_of_value {tau: type} (x: type_denote tau) {struct tau} : val :=
+      let val_of_struct_value :=
+          (fix val_of_struct_value
+               {fields}
+               (x: struct_denote fields)
+           : list val :=
+             match fields return struct_denote fields -> list val with
+             | [] => fun _ => []
+             | (nm, tau) :: fields =>
+               fun '(x, xs) =>
+                 val_of_value x :: (val_of_struct_value xs)
+             end x) in
+      match tau return type_denote tau -> val with
+      | bits_t sz => fun bs => Bits sz  (vect_to_list bs)
+      | enum_t sig => fun bs => Enum sig (vect_to_list bs)
+      | struct_t sig => fun str => Struct sig (val_of_struct_value str)
+      | array_t sig => fun v => Array sig (map val_of_value (vect_to_list v))
+      end x.
+
+    Fixpoint ubits_of_value (v: val) : list bool :=
+      match v with
+      | Bits _ bs => bs
+      | Enum _ bs => bs
+      | Struct _ lv => List.concat (rev (map ubits_of_value lv))
+      | Array _ lv => List.concat (rev (map ubits_of_value lv))
+      end.
+
+    Lemma ubits_of_value_len:
+      forall {tau} (v: type_denote tau) bs,
+        ubits_of_value (val_of_value v) = bs ->
+        List.length bs = type_sz tau.
+    Proof.
+      fix IHt 1. destruct tau; simpl; intros; subst.
+      apply vect_to_list_length.
+      apply vect_to_list_length.
+      - revert sig v. destruct sig. simpl.
+        induction struct_fields; simpl; intros.
+        + subst. reflexivity.
+        + destruct a. destruct v. simpl.
+          rewrite List.concat_app. simpl.
+          rewrite app_length. simpl.
+          rewrite IHstruct_fields.
+          unfold struct_fields_sz. simpl. f_equal.
+          rewrite app_nil_r.
+          eapply IHt; eauto.
+      - revert sig v. destruct sig. simpl. intros.
+        induction array_len; simpl. auto.
+        destruct v. simpl.
+        rewrite concat_app. rewrite app_length. simpl.
+        unfold vect_to_list in IHarray_len. rewrite IHarray_len.
+        clear IHarray_len. f_equal. rewrite app_nil_r. eapply IHt. eauto.
+    Qed.
+
+    Lemma ubits_of_value_ok:
+      forall {tau} (v: type_denote tau) bs,
+        ubits_of_value (val_of_value v) = bs ->
+        vect_to_list (bits_of_value v) = bs.
+    Proof.
+      fix IHt 1. destruct tau; simpl; intros; subst; auto.
+      - revert sig v. destruct sig. simpl.
+        induction struct_fields; simpl; intros.
+        + subst. reflexivity.
+        + destruct a. destruct v. simpl.
+          rewrite List.concat_app. simpl.
+          rewrite <- IHstruct_fields. rewrite app_nil_r.
+          simpl in *.
+          rewrite <- (IHt _ t0 _ eq_refl).
+          rewrite <- vect_to_list_app.
+          reflexivity.
+      - revert sig v. destruct sig. simpl. intros.
+        induction array_len; simpl. auto.
+        destruct v. simpl.
+        rewrite vect_to_list_app. rewrite IHarray_len. clear IHarray_len.
+        rewrite concat_app. f_equal. simpl.
+        rewrite app_nil_r. eapply IHt. eauto.
+    Qed.
+
+
+    Definition bits_split (n: nat) {sz} (v: bits sz)
+      : option (bits n * bits (sz - n)).
+    Proof.
+      destruct (lt_dec n sz). 2: exact None.
+      replace sz with (n + (sz - n)) in v. 2: lia.
+      destruct (Bits.split v) eqn:?.
+      exact (Some (v0, v1)).
+    Defined.
+
+    Fixpoint take_drop {A: Type} (n: nat) (l: list A) : option (list A * list A) :=
+      match n with
+        O => Some ([], l)
+      | S n =>
+        match l with
+          [] => None
+        | a::l =>
+          let/opt2 l1, l2 := take_drop n l in
+          Some (a::l1, l2)
+        end
+      end.
+
+    Definition take_drop' {A: Type} n (l: list A) :=
+      match take_drop n l with
+        None => (l,[])
+      | Some (l1, l2) => (l1, l2)
+      end.
+
+    Fixpoint bits_splitn (nb sz_elt: nat) (bs: list bool)
+      : option (list (list bool))
+      :=
+        match nb with
+          O => Some []
+        | S nb =>
+          let/opt2 hd, rest := take_drop sz_elt bs in
+          let/opt tl := bits_splitn nb sz_elt rest in
+          Some (hd :: tl)
+        end.
+
+    Lemma take_drop_succeeds:
+      forall {A:Type} (n: nat) (l: list A) (LT: n <= Datatypes.length l),
+      exists la lb,
+        take_drop n l = Some (la, lb).
+    Proof.
+      induction n; simpl; intros; eauto.
+      destruct l; simpl in LT. lia.
+      destruct (IHn l) as (la & lb & EQ). lia.
+      rewrite EQ. simpl.
+      eauto.
+    Qed.
+
+    Lemma take_drop_spec:
+      forall {A:Type} (n: nat) (l la lb: list A),
+        take_drop n l = Some (la, lb) ->
+        l = la ++ lb /\ List.length la = n /\ List.length lb = List.length l - n.
+    Proof.
+      induction n; simpl; intros; eauto.
+      inversion H; clear H; subst. repeat split; try reflexivity. lia.
+      destruct l. congruence.
+      destruct (take_drop n l) eqn:EQ; simpl in H; try congruence.
+      destruct p. inversion H; clear H; subst.
+      apply IHn in EQ. destruct EQ as (EQ1 & EQ2 & EQ3). subst. simpl.
+      repeat split; lia.
+    Qed.
+
+    Lemma take_drop'_cons:
+      forall {A} (l l1 l2: list A) a n,
+        take_drop' n l = (l1, l2) ->
+        take_drop' (S n) (a::l) = (a::l1, l2).
+    Proof.
+      unfold take_drop'. simpl. intros. destruct (take_drop n l) eqn:?.
+      - destruct p. inversion H; subst. simpl. auto.
+      - simpl. inversion H; subst. auto.
+    Qed.
+
+    Lemma take_drop'_spec:
+      forall {A:Type} (n: nat) (l la lb: list A),
+        take_drop' n l = (la, lb) ->
+        l = la ++ lb /\ List.length la <= n /\ List.length lb = List.length l - List.length la.
+    Proof.
+      induction n; simpl; intros; eauto.
+      inversion H; clear H; subst. repeat split; try reflexivity. simpl; lia.
+      destruct l; simpl in *. unfold take_drop' in H. simpl in *. inversion H; clear H.
+      simpl. repeat split; lia.
+      destruct (take_drop' n l) as (l1 & l2) eqn:?.
+      erewrite take_drop'_cons in H; eauto. inversion H; subst. simpl.
+      apply IHn in Heqp. destruct Heqp as (EQ1 & EQ2 & EQ3). subst.
+      repeat split; auto. lia.
+    Qed.
+
+
+    Lemma app_eq_inv:
+      forall {A:Type} (a b c d: list A),
+        a ++ b = c ++ d ->
+        List.length a = List.length c ->
+        a = c /\ b = d.
+    Proof.
+      induction a; simpl; intros; eauto.
+      - destruct c; simpl in H0; try congruence.
+        simpl in *. auto.
+      - destruct c; simpl in H0; try congruence.
+        simpl in *. inversion H; clear H; subst.
+        apply IHa in H3. destruct H3; subst; auto. lia.
+    Qed.
+
+    Inductive wt_val: type -> val -> Prop :=
+    | wt_bits: forall n bs,
+        List.length bs = n ->
+        wt_val (bits_t n) (Bits n bs)
+    | wt_enum: forall sig bs,
+        List.length bs = enum_bitsize sig ->
+        wt_val (enum_t sig) (Enum sig bs)
+    | wt_struct: forall sig lv,
+        Forall2 (fun nt v => wt_val nt v) (map snd (struct_fields sig)) lv ->
+        wt_val (struct_t sig) (Struct sig lv)
+    | wt_array: forall sig lv,
+        Forall (fun v => wt_val (array_type sig) v) lv ->
+        List.length lv = array_len sig ->
+        wt_val (array_t sig) (Array sig lv).
+
+    Fixpoint size_type (t: type) :=
+      match t with
+      | bits_t n => 1
+      | enum_t sig => 1
+      | struct_t sig =>
+        1 + list_sum (List.map (fun '(_, t) => size_type t) (struct_fields sig))
+      | array_t sig =>
+        1 + size_type (array_type sig)
+      end.
+
+    Lemma wt_val_ind':
+      forall (P : type -> val -> Prop)
+             (Hbits: forall (n : nat) (bs : list bool), Datatypes.length bs = n -> P (bits_t n) (Bits n bs))
+             (Henum: forall (sig : enum_sig) (bs : list bool),
+                 Datatypes.length bs = enum_bitsize sig -> P (enum_t sig) (Enum sig bs))
+             (Hstruct: forall (sig : struct_sig) (lv : list val),
+                 Forall2 (fun (nt : type) (v : val) => wt_val nt v) (map snd (struct_fields sig)) lv ->
+                 Forall2 (fun (nt : type) (v : val) => wt_val nt v -> P nt v) (map snd (struct_fields sig)) lv ->
+                 P (struct_t sig) (Struct sig lv))
+             (Harray: forall (sig : array_sig) (lv : list val),
+                 Forall (fun v : val => wt_val (array_type sig) v) lv ->
+                 Forall (fun v : val => wt_val (array_type sig) v -> P (array_type sig) v) lv ->
+                 Datatypes.length lv = array_len sig -> P (array_t sig) (Array sig lv)),
+      forall (t : type) (v : val), wt_val t v -> P t v.
+    Proof.
+      intros P Hbits Henum Hstruct Harray t v.
+      remember (size_type t).
+      revert t v Heqn.
+      pattern n.
+      eapply Nat.strong_right_induction with (z:=0).
+      {
+        red. red. intros. subst. tauto.
+      } 2: lia.
+      intros n0 _ Plt t t0 a Heqn.
+      assert (Plt':
+                forall t v,
+                  size_type t < n0 -> wt_val t v -> P t v
+             ).
+      {
+        intros. eapply Plt. 3: reflexivity. lia. auto. auto.
+      } clear Plt.
+      rename Plt' into Plt.
+      subst.
+      inversion Heqn; subst; eauto.
+      - eapply Hstruct. eauto.
+        revert H.
+        simpl in Plt.
+        assert (Forall (fun '(n,t) => forall v, wt_val t v -> P t v) (struct_fields sig)).
+        {
+          revert Plt; clear. destruct sig. simpl.
+          induction struct_fields; simpl; intros. constructor.
+          constructor; eauto. destruct a; simpl; intros.
+          eapply Plt. lia. auto.
+          apply IHstruct_fields.
+          intros; eapply Plt; eauto. lia.
+        }
+        clear Heqn. revert H lv. clear Plt.
+        destruct sig. simpl. clear.
+        induction 1; simpl; intros; eauto. inv H. constructor.
+        inv H1.
+        constructor; auto. destruct x; simpl in *; eauto.
+      - eapply Harray; eauto.
+        rewrite Forall_forall. intros x IN WT.
+        eapply Plt; eauto.
+    Qed.
+
+    Fixpoint size_val (v: val) :=
+      match v with
+      | Bits _ _ => 1
+      | Enum _ _ => 1
+      | Struct sig lv => 1 + list_sum (map size_val lv)
+      | Array sig lv => 1 + list_sum (map size_val lv)
+      end.
+
+
+
+    Lemma take_drop_succeeds_eq:
+      forall {A:Type} (n: nat) (l: list A) (LT: n = Datatypes.length l),
+        take_drop n l = Some (l, []).
+    Proof.
+      induction n; simpl; intros; eauto.
+      destruct l; simpl in LT. reflexivity. lia.
+      destruct l; simpl in LT; try lia.
+      rewrite IHn; simpl; auto.
+    Qed.
+
+    Lemma take_drop_head:
+      forall {A} n (l1 l2: list A),
+        n = List.length l1 ->
+        take_drop n (l1 ++ l2) = Some (l1, l2).
+    Proof.
+      intros. subst. revert l2.
+      induction l1; simpl; intros; subst; eauto.
+      rewrite IHl1. simpl. reflexivity.
+    Qed.
+
+    Lemma length_concat_same:
+      forall {A} (l: list (list A)) sz,
+        Forall (fun x => List.length x = sz) l ->
+        Datatypes.length (List.concat l) = List.length l * sz.
+    Proof.
+      induction 1; simpl; intros; eauto.
+      rewrite app_length; rewrite IHForall. lia.
+    Qed.
+
+
+    Lemma ubits_of_value_len':
+      forall tau v,
+        wt_val tau v ->
+        List.length (ubits_of_value v) = type_sz tau.
+    Proof.
+      intros tau v WT.
+      pattern tau, v.
+      eapply wt_val_ind'; simpl; intros; eauto.
+      - revert sig lv H0 H. destruct sig. simpl.
+        induction struct_fields; simpl; intros.
+        + inv H0. reflexivity.
+        + inv H0. inv H. simpl.
+          rewrite concat_app, app_length. simpl.
+          rewrite app_nil_r. rewrite H3; auto.
+          erewrite IHstruct_fields. reflexivity. eauto. auto.
+      - rewrite Bits.rmul_correct. erewrite length_concat_same.
+        rewrite rev_length. rewrite map_length. rewrite H1. reflexivity.
+        rewrite Forall_forall in *.
+        intros x IN. subst.
+        apply In_rev in IN.
+        rewrite in_map_iff in IN. destruct IN as (x0 & EQ & IN); subst.
+        eapply H0. auto. eauto.
+    Qed.
+
+    Lemma bits_splitn_concat:
+      forall sz l n,
+        Forall (fun l => List.length l = sz) l ->
+        List.length l = n ->
+        bits_splitn n sz (List.concat l) = Some l.
+    Proof.
+      intros. subst.
+      induction H; simpl; intros; auto.
+      rewrite take_drop_head; auto. simpl.
+      rewrite IHForall. simpl. reflexivity.
+    Qed.
+
+
+    Fixpoint uvalue_of_bits {tau: type} (bs: list bool) {struct tau}: option val :=
+      let uvalue_of_struct_bits :=
+          (fix uvalue_of_struct_bits
+               {fields: list (string * type)}
+               (bs: list bool)
+           : option (list val) :=
+             match fields with
+             | [] => Some []
+             | (nm, tau) :: fields =>
+               let/opt2 b0, b1 := take_drop (List.length bs - type_sz tau) bs in
+               let/opt tl := uvalue_of_struct_bits (fields:=fields) b0 in
+               let/opt hd := uvalue_of_bits (tau:=tau) b1 in
+               Some ( hd :: tl)
+             end) in
+      let uvalue_of_list_bits tau :=
+          fix uvalue_of_list_bits (l : list (list bool))
+          : option (list val)
+            :=
+              match l with
+              | [] => Some []
+              | hd::tl =>
+                let/opt hd := uvalue_of_bits (tau:=tau) hd in
+                let/opt tl := uvalue_of_list_bits tl in
+                Some (hd::tl)
+              end in
+      match tau with
+      | bits_t _ => Some (Bits (Datatypes.length bs) bs)
+      | enum_t sig =>
+        let/opt2 b0, b1 := take_drop (enum_bitsize sig) bs in
+        (* TODO check b1 is empty ? *)
+        Some (Enum sig b0)
+      | struct_t sig =>
+        let/opt lv := uvalue_of_struct_bits (fields:=struct_fields sig) bs in
+        Some (Struct sig lv)
+      | array_t sig =>
+        let/opt lbs := bits_splitn (array_len sig)
+                                   (type_sz (array_type sig)) bs in
+        let/opt lv := uvalue_of_list_bits (array_type sig) (rev lbs) in
+        Some (Array sig lv)
+      end
+    .
+
+
+    Lemma uvalue_of_bits_val:
+      forall tau v,
+        wt_val tau v ->
+        uvalue_of_bits (tau:=tau) (ubits_of_value v) =
+        Some v.
+    Proof.
+      intros tau v WT.
+      pattern tau, v.
+      eapply wt_val_ind'; simpl; intros; eauto.
+      - congruence.
+      - rewrite take_drop_succeeds_eq; simpl; auto.
+      - revert sig lv H H0. destruct sig. simpl.
+        induction struct_fields; simpl; intros.
+        + inv H. reflexivity.
+        + inv H. inv H0. destruct a. simpl in *.
+          rewrite concat_app, app_length. simpl. 
+          rewrite app_nil_r.
+          erewrite ubits_of_value_len'. 2: eauto.
+          rewrite take_drop_head. 2: lia. simpl.
+          generalize (IHstruct_fields l' H5 H7). intro A.
+          match type of A with
+            context[ let/opt _ := ?a in _ ] => destruct a eqn:?
+          end; simpl in *; try congruence.
+          rewrite H4. simpl. inv A; auto. auto.
+      -
+        assert (Forall (fun v => wt_val (array_type sig) v /\ uvalue_of_bits (tau:= array_type sig) (ubits_of_value v) = Some v) lv).
+        {
+          rewrite Forall_forall in *; simpl; intros.
+          split; eauto.
+        }
+        clear H H0.
+
+        rewrite bits_splitn_concat.
+        simpl.
+        rewrite rev_involutive.
+        cut ((fix uvalue_of_list_bits (l : list (list bool)) : option (list val) :=
+                match l with
+                | [] => Some []
+                | hd :: tl =>
+                  let/opt hd0 := uvalue_of_bits (tau:=array_type sig) hd
+                  in (let/opt tl0 := uvalue_of_list_bits tl in Some (hd0 :: tl0))
+                end) ((map ubits_of_value lv)) = Some lv).
+        intro A; rewrite A. simpl. reflexivity.
+        revert H1 H2. generalize lv (array_len sig). clear.
+        intros l n EQ. subst. revert l.
+        induction l; simpl; intros; eauto.
+        inv H2. destruct H1. rewrite H0. simpl.
+        rewrite IHl. simpl. auto. auto.
+        rewrite Forall_forall in *. intros x IN.
+        apply In_rev in IN.
+        rewrite in_map_iff in IN. destruct IN as (xx & EQ & IN). subst.
+        erewrite ubits_of_value_len'. eauto.
+        apply H2. auto. rewrite rev_length, map_length; auto.
+    Qed.
+
+    Lemma wt_val_of_value:
+      forall (tau: type) (v: tau),
+        wt_val tau (val_of_value v).
+    Proof.
+      fix IHt 1. destruct tau; simpl; intros.
+      - constructor. rewrite vect_to_list_length. auto.
+      - constructor. rewrite vect_to_list_length. auto.
+      - eapply wt_struct.
+        revert v. generalize (struct_fields sig).
+        induction l; simpl; intros; eauto.
+        destruct a. destruct v. simpl. constructor. apply IHt.
+        eauto.
+      - eapply wt_array.
+        rewrite Forall_forall. intros x IN.
+        rewrite in_map_iff in IN.
+        destruct IN as (xx & EQ & IN). subst.
+        apply IHt.
+        rewrite map_length.
+        rewrite vect_to_list_length. auto.
+    Qed.
+
+
+    Lemma uvalue_of_bits_val':
+      forall tau v,
+        uvalue_of_bits (tau:=tau) (ubits_of_value (val_of_value (tau:=tau) v)) =
+        Some (val_of_value (tau:=tau) v).
+    Proof.
+      intros.
+      apply uvalue_of_bits_val.
+      apply wt_val_of_value.
+    Qed.
+
+
+    Fixpoint get_field_struct (s: list (string * type)) (lv: list val) f : option val :=
+      match s, lv with
+      | (n, _)::s, a::lv =>
+        if eq_dec n f
+        then Some a
+        else get_field_struct s lv f
+      | _, _ => None
+      end.
+
+
+    Fixpoint find_field_offset_right (s: list (string * type)) f : option (nat * nat) :=
+      match s with
+      | (n, t)::s =>
+        if eq_dec f n
+        then
+          Some (struct_fields_sz s, type_sz t)
+        else
+          find_field_offset_right s f
+      | [] => None
+      end.
+
+    Definition get_field (s: val) f : option val :=
+      match s with
+        Struct sig lv =>
+        get_field_struct (struct_fields sig) lv f
+      | _ => None
+      end.
+
+
+
+    Lemma uvalue_of_bits_val_of_value:
+      forall (tau: type) (v: vect bool (type_sz tau)),
+        uvalue_of_bits (tau:=tau) (vect_to_list v) = Some (val_of_value (value_of_bits v)).
+    Proof.
+      intros; rewrite <- uvalue_of_bits_val'. f_equal.
+      erewrite <- ubits_of_value_ok. 2: eauto.
+      rewrite bits_of_value_of_bits. auto.
+    Qed.
+
+    Lemma repeat_bits_const:
+      forall x n,
+        repeat x n = vect_to_list (Bits.const n x).
+    Proof.
+      induction n; simpl; auto.
+      rewrite IHn. reflexivity.
+    Qed.
+
+    Lemma last_nth:
+      forall {A} d (l: list A),
+        last l d = nth (List.length l - 1) l d.
+    Proof.
+      induction l; simpl; intros; eauto.
+      destr. simpl. auto.
+      rewrite IHl. simpl. rewrite Nat.sub_0_r. reflexivity.
+    Qed.
+
+    Lemma bits_nth_list:
+      forall s (v: vect bool s) idx,
+        Bits.nth v idx = nth (index_to_nat idx) (vect_to_list v) false.
+    Proof.
+      induction s; intros. simpl in idx; easy.
+      unfold Bits.nth. destr. simpl. auto. fold @vect_nth.
+      rewrite IHs. destruct v.  simpl. reflexivity.
+    Qed.
+
+    Lemma msb_spec:
+      forall s (v: bits s),
+        Bits.msb v = last (vect_to_list v) false.
+    Proof.
+      unfold Bits.msb. intros.
+      destr. destruct v. reflexivity.
+      rewrite vect_last_nth.
+      rewrite last_nth. rewrite vect_to_list_length.
+      simpl Nat.sub.
+      rewrite Nat.sub_0_r.
+      rewrite bits_nth_list. f_equal.
+      apply index_to_nat_of_nat.
+      apply index_of_nat_largest.
+    Qed.
+
+
+    Lemma vect_extend_end_firstn:
+      forall x s' (v: bits (Nat.min x s')) d,
+        vect_to_list (vect_extend_end_firstn v d) =
+        vect_to_list (vect_extend_end v x d).
+    Proof.
+      unfold vect_extend_end_firstn.
+      intros. rewrite vect_to_list_eq_rect. auto.
+    Qed.
+
+    Lemma vect_to_list_cons:
+      forall {A: Type} e s (v: vect A s),
+        vect_to_list (e::v)%vect = e:: vect_to_list v.
+    Proof.
+      reflexivity.
+    Qed.
+
+    Lemma vect_firstn_to_list:
+      forall s (v: bits s) n,
+        vect_to_list (vect_firstn n v) = fst (take_drop' n (vect_to_list v)).
+    Proof.
+      induction s; simpl; intros. simpl in *. destruct v. destr; reflexivity.
+      destr. reflexivity.
+      erewrite <- vect_to_list_eq_rect.
+      Unshelve.
+      3: replace (Nat.min (S n0) (S s)) with (S (Nat.min n0 s)); reflexivity.
+      simpl.
+      rewrite vect_to_list_cons.
+      rewrite IHs.
+      destruct v. simpl.
+      cbn. unfold take_drop'. simpl. unfold vect_to_list.
+      destr. destruct p. simpl. reflexivity.
+      simpl. reflexivity.
+    Qed.
+
+    Lemma vect_skipn_to_list:
+      forall s (v: bits s) n,
+        vect_to_list (vect_skipn n v) = snd (take_drop' n (vect_to_list v)).
+    Proof.
+      induction s; simpl; intros. simpl in *. destruct v. destr; reflexivity.
+      destr. reflexivity.
+      rewrite IHs.
+      unfold take_drop'.
+      destruct v. simpl.
+      cbn. unfold vect_to_list.
+      destr. destruct p. simpl. reflexivity.
+      simpl. reflexivity.
+    Qed.
+
+    Lemma take_drop'_spec2:
+      forall {A:Type} (n: nat) (l la lb: list A),
+        take_drop' n l = (la, lb) ->
+        l = la ++ lb /\
+        List.length la = Nat.min n (List.length l).
+    Proof.
+      induction n; simpl; intros; eauto.
+      inversion H; clear H; subst. repeat split; try reflexivity.
+      destruct l; simpl in *. unfold take_drop' in H. simpl in *. inversion H; clear H.
+      simpl. repeat split; lia.
+      destruct (take_drop' n l) as (l1 & l2) eqn:?.
+      erewrite take_drop'_cons in H; eauto. inv H. simpl.
+      apply IHn in Heqp. destruct Heqp as (EQ1 & EQ2). subst.
+      repeat split; auto.
+    Qed.
+
+    Lemma struct_fields_sz_skipn:
+      forall n f,
+        struct_fields_sz (skipn n f) <= struct_fields_sz f.
+    Proof.
+      induction n; simpl; intros; eauto. destr. auto.
+      etransitivity. apply IHn. unfold struct_fields_sz. simpl. lia.
+    Qed.
+    Lemma field_offset_right_le:
+      forall sig s,
+        field_offset_right sig s <= struct_sz sig.
+    Proof.
+      unfold field_offset_right, struct_sz.
+      simpl type_sz.
+      intros; apply struct_fields_sz_skipn.
+    Qed.
+
+
+    Lemma find_field_offset_right_spec:
+      forall f sig (i: index (List.length (struct_fields sig))),
+        PrimTypeInference.find_field sig f = Success i ->
+        find_field_offset_right (struct_fields sig) f = Some (field_offset_right sig i, field_sz sig i).
+    Proof.
+      intros f sig i FF.
+      unfold PrimTypeInference.find_field in FF. unfold opt_result in FF.
+      destr_in FF; inv FF.
+      revert i Heqo. simpl. destruct sig. simpl. clear.
+      induction struct_fields; intros; eauto. easy.
+      simpl. destruct a. simpl in *.
+      destr_in Heqo.
+      * inv Heqo. f_equal.
+      * destr_in Heqo; inv Heqo.
+        erewrite IHstruct_fields; eauto.
+        f_equal.
+    Qed.
+
+
+    Definition enum_sig_eq_dec (s1 s2: enum_sig) : {s1 = s2} + {s1 <> s2}.
+    Proof.
+      destruct s1, s2; simpl.
+      destruct (eq_dec enum_name enum_name0). 2: right; intro A; inv A; congruence.
+      destruct (eq_dec enum_size enum_size0). 2: right; intro A; inv A; congruence.
+      destruct (eq_dec enum_bitsize enum_bitsize0). 2: right; intro A; inv A; congruence.
+      subst.
+      destruct (eq_dec enum_members enum_members0).
+      destruct (eq_dec enum_bitpatterns enum_bitpatterns0).
+      left; subst; reflexivity. right; intro A; inv A.
+      apply Eqdep_dec.inj_pair2_eq_dec in H1. 2: apply eq_dec.
+      apply Eqdep_dec.inj_pair2_eq_dec in H1. 2: apply eq_dec.
+      congruence.
+      right; intro A; inv A.
+      apply Eqdep_dec.inj_pair2_eq_dec in H0. 2: apply eq_dec. congruence.
+    Defined.
+
+
+    Definition struct_sig_eq_dec (s1 s2: struct_sig) : {s1 = s2} + {s1 <> s2}.
+    Proof.
+      destruct s1, s2; simpl.
+      destruct (eq_dec struct_name struct_name0). 2: right; intro A; inv A; congruence.
+      destruct (eq_dec struct_fields struct_fields0). 2: right; intro A; inv A; congruence.
+      left; subst; reflexivity.
+    Defined.
+
+    Lemma strong_ind_type:
+      forall (P: nat -> Type)
+             (IH: forall n, (forall m, m < n -> P m) -> P n),
+      forall n, forall m, m <= n -> P m.
+    Proof.
+      induction n. intros. apply IH. lia.
+      intros.
+      destruct (le_dec m n); eauto.
+      assert (m = S n) by lia. clear H n0. subst.
+      apply IH. intros. apply IHn; auto. lia.
+    Qed.
+
+    Lemma val_ind':
+      forall (P : val -> Type)
+             (Hbits: forall (n : nat) (bs : list bool), P (Bits n bs))
+             (Henum: forall (sig : enum_sig) (bs : list bool),
+                 P (Enum sig bs))
+             (Hstruct: forall (sig : struct_sig) (lv : list val),
+                 (forall x, In x lv -> P x) ->
+                 P (Struct sig lv))
+             (Harray: forall (sig : array_sig) (lv : list val),
+                 (forall x, In x lv -> P x) ->
+                 P (Array sig lv)),
+      forall (v : val), P v.
+    Proof.
+      intros P Hbits Henum Hstruct Harray v.
+      remember (size_val v).
+      revert v Heqn.
+      pattern n.
+      eapply strong_ind_type. 2: reflexivity.
+      intros n0 Plt v Heqn.
+      assert (Plt':
+                forall v,
+                  size_val v < n0 -> P v
+             ).
+      {
+        intros. eapply Plt. 2: reflexivity. lia.
+      } clear Plt.
+      rename Plt' into Plt.
+      subst.
+      destruct v; eauto.
+      - eapply Hstruct.
+        intros.
+        eapply Plt. simpl.
+        clear Plt. revert x v H.
+        induction v; simpl; intros; eauto. easy.
+        destruct H; subst; eauto. lia.
+        eapply lt_le_trans. apply IHv; auto. lia.
+      - eapply Harray.
+        intros.
+        eapply Plt. simpl.
+        clear Plt. revert x v H.
+        induction v; simpl; intros; eauto. easy.
+        destruct H; subst; eauto. lia.
+        eapply lt_le_trans. apply IHv; auto. lia.
+    Qed.
+
+    Definition list_eq_dec' {A: Type} (l1 l2: list A) (Aeq: forall x y, In x l1 -> {x = y} + {x <> y}): {l1 = l2} + {l1 <> l2}.
+    Proof.
+      revert l1 Aeq l2; induction l1; simpl; intros.
+      - destruct l2. left; reflexivity. right; intro B; inv B.
+      - destruct l2. right; congruence.
+        destruct (Aeq a a0). simpl; auto. subst.
+        2: right; intro B; inv B; congruence.
+        edestruct (fun pf => IHl1 pf l2). intros; eauto.
+        subst. left; reflexivity.
+        right; intro B; inv B; congruence.
+    Defined.
+
+    Definition val_eq_dec (v1 v2: val) : {v1 = v2} + {v1 <> v2}.
+    Proof.
+      revert v2.
+      pattern v1. revert v1.
+      eapply val_ind'; simpl; intros.
+      - destruct v2; try (right; intro A; inv A; congruence).
+        destruct (eq_dec n sz); try (right; intro A; inv A; congruence).
+        destruct (eq_dec bs v); try (right; intro A; inv A; congruence).
+        subst; left; reflexivity.
+      - destruct v2; try (right; intro A; inv A; congruence).
+        destruct (enum_sig_eq_dec sig sig0); try (right; intro A; inv A; congruence).
+        destruct (eq_dec bs v); try (right; intro A; inv A; congruence).
+        subst; left; reflexivity.
+      - destruct v2; try (right; intro A; inv A; congruence).
+        destruct (struct_sig_eq_dec sig sig0); try (right; intro A; inv A; congruence).
+        destruct (list_eq_dec' lv v); try (right; intro A; inv A; congruence). eauto.
+        left; subst. reflexivity.
+      - destruct v2; try (right; intro A; inv A; congruence).
+        destruct (eq_dec sig sig0); subst. 2: (right; intro A; inv A; congruence).
+        destruct (list_eq_dec' lv v); try (right; intro A; inv A; congruence). eauto.
+        left; subst. reflexivity.
+    Defined.
+
+    Fixpoint bitwise (f: bool -> bool -> bool) (l1 l2: list bool) {struct l1}: list bool :=
+      match l1, l2 with
+      | [], [] => []
+      | [], l2 => map (fun x => f false x) l2
+      | l1, [] => map (fun x => f x false) l1
+      | a1::l1, a2::l2 => f a1 a2 :: bitwise f l1 l2
+      end.
+
+    Lemma and_correct:
+      forall sz (arg1: arg1Sig (PrimSignatures.Sigma2 (PrimTyped.Bits2 (PrimTyped.And sz))))
+             (arg2: arg2Sig (PrimSignatures.Sigma2 (PrimTyped.Bits2 (PrimTyped.And sz)))) ret,
+        PrimSpecs.sigma2 (PrimTyped.Bits2 (PrimTyped.And sz)) arg1 arg2 = ret ->
+        match val_of_value arg1, val_of_value arg2 with
+        | Bits _ arg1, Bits _ arg2 =>
+          exists sz, Bits sz (bitwise andb arg1 arg2) = (val_of_value ret)
+        | _, _ => False
+        end.
+    Proof.
+      simpl. intros. eexists. f_equal. subst.
+      revert arg1 arg2.
+      induction sz; simpl. reflexivity.
+      destruct arg1, arg2. simpl.
+      unfold Bits.and in *. simpl.
+      rewrite vect_to_list_cons. f_equal. rewrite <- IHsz.
+      reflexivity.
+    Qed.
+
+
+    Lemma len_to_list: forall sz (v: bits sz), sz = Datatypes.length (vect_to_list v).
+    Proof.
+      intros; rewrite vect_to_list_length. reflexivity.
+    Defined.
+
+    Lemma vect_to_list_of_list:
+      forall (v: list bool),
+        vect_to_list (vect_of_list v) = v.
+    Proof.
+      induction v; simpl; intros. reflexivity.
+      rewrite vect_to_list_cons. congruence.
+    Qed.
+
+    Lemma vect_of_list_to_list:
+      forall sz (v: bits sz),
+        vect_of_list (vect_to_list v) = rew [vect bool] (len_to_list sz v) in v.
+    Proof.
+      intros. apply vect_to_list_inj.
+      rewrite vect_to_list_of_list.
+      rewrite vect_to_list_eq_rect. reflexivity.
+    Qed.
+
+
+    Lemma vect_to_list_vect_unsnoc:
+      forall sz (v: bits (S sz)) b v',
+        vect_unsnoc v = (b, v') ->
+        vect_to_list v' = removelast (vect_to_list v).
+    Proof.
+      induction sz; simpl; intros.
+      - inv H. destruct v. simpl. reflexivity.
+      - destr_in H. inv H.
+        rewrite vect_to_list_cons. f_equal.
+        erewrite IHsz. 2: eauto. simpl. reflexivity.
+    Qed.
+
+
+    Lemma lsl1:
+      forall sz (v: bits sz),
+        sz <> 0 ->
+        vect_to_list (Bits.lsl1 v) = false :: removelast (vect_to_list v).
+    Proof.
+      unfold Bits.lsl1. destruct sz. congruence. intros.
+      rewrite vect_to_list_cons. f_equal.
+      erewrite vect_to_list_vect_unsnoc. 2: apply surjective_pairing.
+      reflexivity.
+    Qed.
+
+    Lemma lsl1':
+      forall sz (v: bits sz),
+        vect_to_list (Bits.lsl1 v) = if eq_dec sz O then [] else false :: removelast (vect_to_list v).
+    Proof.
+      intros. destr.
+      subst. destruct v; reflexivity.
+      apply lsl1; auto.
+    Qed.
+
+    Lemma and_correct':
+      forall sz (arg1: bits_t sz)
+             (arg2: bits_t sz),
+        bitwise andb (vect_to_list arg1) (vect_to_list arg2) = vect_to_list (Bits.and arg1 arg2).
+    Proof.
+      induction sz; simpl. reflexivity.
+      destruct arg1, arg2. simpl.
+      unfold Bits.and in *. simpl.
+      rewrite vect_to_list_cons. f_equal. rewrite <- IHsz.
+      reflexivity.
+    Qed.
+
+
+    Lemma or_correct':
+      forall sz (arg1: bits_t sz)
+             (arg2: bits_t sz),
+        bitwise orb (vect_to_list arg1) (vect_to_list arg2) = vect_to_list (Bits.or arg1 arg2).
+    Proof.
+      induction sz; simpl. reflexivity.
+      destruct arg1, arg2. simpl.
+      unfold Bits.or in *. simpl.
+      rewrite vect_to_list_cons. f_equal. rewrite <- IHsz.
+      reflexivity.
+    Qed.
+
+
+    Lemma xor_correct':
+      forall sz (arg1: bits_t sz)
+             (arg2: bits_t sz),
+        bitwise xorb (vect_to_list arg1) (vect_to_list arg2) = vect_to_list (Bits.xor arg1 arg2).
+    Proof.
+      induction sz; simpl. reflexivity.
+      destruct arg1, arg2. simpl.
+      unfold Bits.xor in *. simpl.
+      rewrite vect_to_list_cons. f_equal. rewrite <- IHsz.
+      reflexivity.
+    Qed.
+
+    Lemma iter_assoc_spec:
+      forall {A:Type} (f: A -> A) n x,
+        Nat.iter n f (f x) = f (Nat.iter n f x).
+    Proof.
+      induction n; simpl; intros; eauto.
+      rewrite IHn. auto.
+    Qed.
+    
+    Lemma vect_dotimes_spec:
+      forall {A:Type} (f: A -> A) n x,
+        vect_dotimes f n x = Nat.iter n f x.
+    Proof.
+      induction n; simpl; intros. auto.
+      rewrite IHn, iter_assoc_spec. auto.
+    Qed.
+
+    Lemma vect_to_list_snoc:
+      forall sz (v: bits sz) x,
+        vect_to_list (vect_snoc x v) = vect_to_list v ++ [x].
+    Proof.
+      induction sz; simpl; intros; eauto.
+      rewrite vect_to_list_cons. f_equal.
+      rewrite IHsz. reflexivity.
+    Qed.
+    
+    Lemma lsr1:
+      forall sz (v: bits sz),
+        sz <> 0 ->
+        vect_to_list (Bits.lsr1 v) = tl (vect_to_list v) ++ [false].
+    Proof.
+      unfold Bits.lsr1. intros. destr.
+      rewrite vect_to_list_snoc.
+      rewrite <- (vect_cons_hd_tl v) at 2.
+      rewrite vect_to_list_cons. simpl. reflexivity.
+    Qed.
+
+    Lemma asr1:
+      forall sz (v: bits sz),
+        sz <> 0 ->
+        vect_to_list (Bits.asr1 v) = tl (vect_to_list v) ++ [last (vect_to_list v) false].
+    Proof.
+      unfold Bits.asr1. intros. destr.
+      rewrite vect_to_list_snoc. f_equal.
+      rewrite msb_spec. auto.
+    Qed.
+    
+    Lemma iter_list_vect:
+      forall sz (v: bits sz) (f: list bool -> list bool) (g: bits sz -> bits sz),
+        (forall x, f (vect_to_list x) = vect_to_list (g x)) ->
+        forall n,
+          Nat.iter n f (vect_to_list v) = vect_to_list (vect_dotimes g n v).
+    Proof.
+      intros. rewrite vect_dotimes_spec. induction n; simpl; intros; eauto.
+      rewrite IHn. apply H.
+    Qed.
+
+    Lemma sel:
+      forall sz (bs: bits sz) idx,
+        vect_to_list (BitFuns.sel bs idx) =
+        [List.nth (Bits.to_nat idx) (vect_to_list bs) false].
+    Proof.
+      unfold BitFuns.sel. intros.
+      destr.
+      rewrite bits_nth_list. unfold Bits.to_index in Heqo.
+      erewrite index_to_nat_of_nat. 2: eauto. reflexivity.
+      unfold Bits.to_index in Heqo.
+      rewrite nth_overflow. reflexivity.
+      rewrite vect_to_list_length.
+      apply index_of_nat_none_ge in Heqo. lia.
+    Qed.
+    Lemma slice_subst:
+      forall sz (bs: bits sz) ofs w v,
+        vect_to_list (Bits.slice_subst ofs w bs v) =
+        let '(h, _) := take_drop' ofs (vect_to_list bs) in
+        let '(_, t) := take_drop' (ofs + w) (vect_to_list bs) in
+        fst (take_drop' sz (h ++ (vect_to_list v) ++ t)).
+    Proof.
+      unfold Bits.slice_subst. intros.
+      destr. destr.
+      rewrite vect_to_list_eq_rect.
+      rewrite vect_firstn_to_list. f_equal.
+      rewrite ! vect_to_list_app.
+      rewrite vect_firstn_to_list. f_equal.
+      rewrite Heqp. simpl. f_equal.
+      rewrite vect_skipn_to_list. rewrite Heqp0. reflexivity.
+    Qed.
+
+    Lemma slice:
+      forall sz (bs: bits sz) ofs w,
+        vect_to_list (Bits.slice ofs w bs) =
+        let '(_, bs) := take_drop' ofs (vect_to_list bs) in
+        let '(bs, _) := take_drop' w bs in
+        (bs ++ List.repeat false (w - Nat.min w (sz - ofs))).
+    Proof.
+      intros. unfold Bits.slice. rewrite vect_extend_end_firstn.
+      unfold Bits.extend_end.
+      rewrite vect_to_list_eq_rect.
+      rewrite vect_to_list_app.
+      rewrite vect_firstn_to_list.
+      rewrite vect_skipn_to_list.
+      rewrite <- repeat_bits_const.
+      destr. simpl. destr. simpl.
+      f_equal.
+    Qed.
+    Lemma vect_to_list_eq:
+      forall sz1 sz2 (v1: bits sz1) (v2: bits sz2) (pf: sz1 = sz2),
+        rew [fun x => bits x] pf in v1 = v2 ->
+                                    vect_to_list v1 = vect_to_list v2.
+    Proof.
+      intros. subst. rewrite vect_to_list_eq_rect. auto.
+    Qed.
+
+    Lemma bits_map_rew:
+      forall sz1 sz2 (v: bits sz1) f (pf: sz1 = sz2),
+        Bits.map f (rew [Bits.bits] pf in v) = rew [Bits.bits] pf in (Bits.map f v).
+    Proof.
+      intros. subst. simpl. auto.
+    Qed.
+
+    Lemma cmp:
+      forall sz (v1 v2: bits sz) c,
+        vect_to_list (BitFuns.bitfun_of_predicate c v1 v2) =
+        [c v1 v2].
+    Proof.
+      unfold BitFuns.bitfun_of_predicate. simpl; intros. reflexivity.
+    Qed.
+    Lemma lift_comparison_rew:
+      forall {A} sz1 sz1' (pf: sz1 = sz1') (pf2: sz1 = sz1') (v1: bits sz1) (v2: bits sz1) (cast: forall sz, bits sz -> A) compare cmp,
+        Bits.lift_comparison (cast sz1') compare cmp (rew [Bits.bits] pf in v1) (rew [Bits.bits] pf2 in v2) =
+        Bits.lift_comparison (cast sz1) compare cmp v1 v2.
+    Proof.
+      intros. subst. simpl.
+      rewrite (Eqdep_dec.UIP_refl_nat _ pf2). simpl. reflexivity.
+    Qed.
+
+
+    Fixpoint subst_field (n: nat) (v: val) (s: list val) : option (list val) :=
+      match n, s with
+      | _, [] => None
+      | O, a::r => Some (v::r)
+      | S n, a::r => let/opt s := subst_field n v r in Some (a::s)
+      end.
+
+    Fixpoint val_of_struct_value'
+             (fields : list (string * type))
+             (x : struct_denote fields)
+             {struct fields} : list val :=
+      match fields as fields0 return (struct_denote fields0 -> list val) with
+      | [] => fun _ : unit => []
+      | p :: fields0 =>
+        let (_, tau) as p0 return (snd p0 * struct_denote fields0 -> list val) := p in
+        fun '(x0, xs) => val_of_value x0 :: val_of_struct_value' fields0 xs
+      end x.
+
+    Lemma val_of_struct_value_rew:
+      forall fields x,
+        (fix
+           val_of_struct_value (fields : list (string * type)) (x : struct_denote fields) {struct
+                                                                                             fields} : list val :=
+           match fields as fields0 return (struct_denote fields0 -> list val) with
+           | [] => fun _ : unit => []
+           | p :: fields0 =>
+             let (_, tau) as p0 return (snd p0 * struct_denote fields0 -> list val) := p in
+             fun '(x0, xs) => val_of_value x0 :: val_of_struct_value fields0 xs
+           end x) fields x =
+        val_of_struct_value' fields x.
+    Proof.
+      induction fields; simpl; intros; eauto.
+    Qed.
+
+    Lemma subst_field_ok':
+      forall flds idx v s,
+        subst_field (index_to_nat idx) (val_of_value v)
+                    (val_of_struct_value' flds s) =
+        Some (val_of_struct_value' flds
+                                   (BitFuns.subst_field flds s idx v)).
+    Proof.
+      induction flds; simpl; intros; eauto. easy.
+      repeat destr. simpl in *. auto.
+      simpl in *. rewrite IHflds. simpl. auto.
+    Qed.
+
+    Lemma subst_field_ok:
+      forall sig idx (s: struct_t sig) v,
+      exists s',
+        val_of_value s = Struct sig s' /\
+        exists s'',
+          subst_field (index_to_nat idx) (val_of_value v) s' = Some s'' /\
+          Struct sig s'' =
+          val_of_value (tau:=struct_t sig) (BitFuns.subst_field (struct_fields sig) s idx v)
+    .
+    Proof.
+      intros.
+      simpl in s.
+      revert s idx v. simpl. intros.
+      rewrite ! val_of_struct_value_rew.
+      eexists; split; eauto.
+      rewrite subst_field_ok'.
+      eexists; split; eauto.
+    Qed.
+
+    Fixpoint subst_field_name (flds: list (string * type)) (n: string)
+             (v: val) (s: list val) : option (list val) :=
+      match flds, s with
+      | _, [] => None
+      | [], _ => None
+      | (name, _)::flds, a::r =>
+        if eq_dec n name then Some (v::r)
+        else let/opt s := subst_field_name flds n v r in Some (a::s)
+      end.
+
+
+    Lemma subst_field_name_ok':
+      forall flds x idx fname v s,
+        PrimTypeInference.find_field {| struct_name := x; struct_fields := flds|} fname = Success idx ->
+        subst_field_name flds fname (val_of_value v)
+                         (val_of_struct_value' flds s) =
+        Some (val_of_struct_value' flds
+                                   (BitFuns.subst_field flds s idx v)).
+    Proof.
+      induction flds; simpl; intros; eauto. easy.
+      destr_in v.
+      - destruct a. destruct s. simpl in *.
+        unfold PrimTypeInference.find_field in H. simpl in H.
+        destr_in H.
+        + subst. simpl in H. inv H. auto.
+        + destr_in H; inv H.
+      - destruct a, s.
+        unfold PrimTypeInference.find_field in H. simpl in H.
+        destr_in H.
+        + subst. simpl in H. inv H.
+        + destr_in H; inv H. simpl in *. erewrite IHflds with (x:=x). simpl. auto.
+          unfold PrimTypeInference.find_field. simpl. rewrite Heqo. simpl. auto.
+    Qed.
+
+    Lemma subst_field_name_ok:
+      forall sig fname idx (s: struct_t sig) v,
+        PrimTypeInference.find_field sig fname = Success idx ->
+        exists s',
+          val_of_value s = Struct sig s' /\
+          exists s'',
+            subst_field_name (struct_fields sig) fname (val_of_value v) s' = Some s'' /\
+            Struct sig s'' =
+            val_of_value (tau:=struct_t sig) (BitFuns.subst_field (struct_fields sig) s idx v)
+    .
+    Proof.
+      intros.
+      simpl in s.
+      revert s idx v H. simpl. intros.
+      rewrite ! val_of_struct_value_rew.
+      eexists; split; eauto.
+      erewrite subst_field_name_ok'.
+      eexists; split; eauto.
+      instantiate(1:= struct_name sig).
+      destruct sig. eauto.
+    Qed.
+
+    Lemma vect_replace_to_list:
+      forall {A: Type} sz (v: vect A sz) l1 (a: A) l2 x idx,
+        vect_to_list v = l1 ++ a :: l2 ->
+        List.length l1 = index_to_nat idx ->
+        vect_to_list (vect_replace v idx x) = l1 ++ x :: l2.
+    Proof.
+      induction sz; simpl; intros; eauto. easy.
+      destr.
+      - destruct l1; simpl in *; try lia. subst.
+        rewrite vect_to_list_cons. f_equal.
+        destruct v; simpl in *.
+        unfold vect_to_list in H. simpl in H. inv H. reflexivity.
+      - rewrite vect_to_list_cons. subst. simpl.
+        destruct v; simpl in *.
+        unfold vect_to_list in H. simpl in H. fold (@vect_to_list A) in H.
+        destruct l1. simpl in *. lia. simpl in H. inv H.
+        simpl. f_equal. simpl in H0. inv H0.
+        eapply IHsz; eauto.
+    Qed.
+
+    Lemma take_drop_map:
+      forall {A B: Type} (f: A -> B) n l l1 l2,
+        take_drop n (map f l) = Some (l1, l2) ->
+        exists l1' l2',
+          take_drop n l = Some (l1', l2') /\
+          l1 = List.map f l1' /\
+          l2 = List.map f l2'.
+    Proof.
+      induction n; simpl; intros; eauto.
+      - inv H. exists [], l; repeat split; eauto.
+      - destr_in H. inv H.
+        destruct (take_drop n l0) eqn:?; try congruence. 2: inv H.
+        destruct p; simpl in *. inv H.
+        destr. simpl in *. congruence. simpl in *. inv Heql0.
+        edestruct IHn as (l1' & l2' & EQ1 & EQ2 & EQ3). eauto.
+        rewrite EQ1. simpl. (do 2 eexists); repeat split; eauto.
+        subst; reflexivity.
+    Qed.
+
+        Fixpoint list_assoc {K V: Type} {eq: EqDec K} (l: list (K * V)) (k: K): option V :=
+      match l with
+        [] => None
+      | (k1,v1)::l =>
+        if eq_dec k k1 then Some v1 else list_assoc  l k
+      end.
+
+    Fixpoint list_assoc_set {K V: Type} {eq: EqDec K} (l: list (K * V)) (k: K) (v: V): list (K * V) :=
+      match l with
+        [] => [(k,v)]
+      | (k1,v1)::l =>
+        if eq_dec k k1 then (k1,v)::l else (k1,v1) :: list_assoc_set l k v
+      end.
+
+
+    
+    Fixpoint uvalue_of_struct_bits
+             (fields: list (string * type))
+             (bs: list bool)
+      : option (list val) :=
+      match fields with
+      | [] => Some []
+      | (nm, tau) :: fields =>
+        let/opt2 b0, b1 := take_drop (List.length bs - type_sz tau) bs in
+        let/opt tl := uvalue_of_struct_bits fields b0 in
+        let/opt hd := uvalue_of_bits (tau:=tau) b1 in
+        Some ( hd :: tl)
+      end.
+
+    Fixpoint uvalue_of_list_bits
+             {tau}
+             (bs: list (list bool))
+      : option (list val) :=
+      match bs with
+      | [] => Some []
+      | l :: bs =>
+        let/opt hd0 := uvalue_of_bits (tau:=tau) l in
+        let/opt tl0 := uvalue_of_list_bits (tau:=tau) bs in
+        Some (hd0 :: tl0)
+      end.
+
+
+    
+
